thys/Pi_Calculus/Commitment.thy
@@ -4,10 +4,10 @@ begin
 
 local_setup \<open>fn lthy =>
 let
-  val name1 = "Com_internal"
-  val name2 = "Com"
-  val T1 = @{typ "'var Proc"}
-  val T2 = @{typ "'var * 'var * 'var Proc +'var * 'var * 'var Proc + 'var * 'bvar * 'brec + 'var Proc + 'var * 'bvar * 'brec"}
+  val name1 = "comP_internal"
+  val name2 = "comP"
+  val T1 = @{typ "'var procP"}
+  val T2 = @{typ "'var * 'var * 'var procP +'var * 'var * 'var procP + 'var * 'bvar * 'brec + 'var procP + 'var * 'bvar * 'brec"}
   val Xs = map dest_TFree []
   val resBs = map dest_TFree [@{typ 'var}, @{typ 'bvar}, @{typ 'brec}, @{typ 'rec}]
   val rel = [[0]]
@@ -46,255 +46,255 @@ print_theorems
 
 
 (* Monomorphization: *)
-type_synonym com = "var Com"
-instance var :: var_Com_pre by standard
-instance var :: var_Com_internal_pre by standard
+type_synonym com = "var comP"
+instance var :: var_comP_pre by standard
+instance var :: var_comP_internal_pre by standard
 
 definition Finp :: "var \<Rightarrow> var \<Rightarrow> proc \<Rightarrow> com" where
-  "Finp x y t \<equiv> Com_ctor (Abs_Com_pre (Inl (x, y, t)))"
+  "Finp x y t \<equiv> comP_ctor (Abs_comP_pre (Inl (x, y, t)))"
 definition Fout :: "var \<Rightarrow> var \<Rightarrow> proc \<Rightarrow> com" where
-  "Fout x y t \<equiv> Com_ctor (Abs_Com_pre (Inr (Inl (x, y, t))))"
+  "Fout x y t \<equiv> comP_ctor (Abs_comP_pre (Inr (Inl (x, y, t))))"
 definition Bout :: "var \<Rightarrow> var \<Rightarrow> proc \<Rightarrow> com" where
-  "Bout x y t \<equiv> Com_ctor (Abs_Com_pre (Inr (Inr (Inl (x, y, Com_internal_ctor (Abs_Com_internal_pre t))))))"
+  "Bout x y t \<equiv> comP_ctor (Abs_comP_pre (Inr (Inr (Inl (x, y, comP_internal_ctor (Abs_comP_internal_pre t))))))"
 definition Tau :: "proc \<Rightarrow> com" where
-  "Tau t \<equiv> Com_ctor (Abs_Com_pre (Inr (Inr (Inr (Inl t)))))"
+  "Tau t \<equiv> comP_ctor (Abs_comP_pre (Inr (Inr (Inr (Inl t)))))"
 definition Binp :: "var \<Rightarrow> var \<Rightarrow> proc \<Rightarrow> com" where
-  "Binp x y t \<equiv> Com_ctor (Abs_Com_pre (Inr (Inr (Inr (Inr (x, y, Com_internal_ctor (Abs_Com_internal_pre t)))))))"
+  "Binp x y t \<equiv> comP_ctor (Abs_comP_pre (Inr (Inr (Inr (Inr (x, y, comP_internal_ctor (Abs_comP_internal_pre t)))))))"
 
-lemmas toUnfold = set1_Com_internal_pre_def
+lemmas toUnfold = set1_comP_internal_pre_def
   UN_empty UN_empty2 UN_single Un_empty_left Un_empty_right
   comp_def empty_Diff
   map_prod_simp prod_set_simps
   map_sum.simps sum_set_simps prod_set_simps
   Sup_empty cSup_singleton
   (* *)
-  Abs_Com_pre_inverse[OF UNIV_I]
-  set1_Com_pre_def set2_Com_pre_def set4_Com_pre_def set3_Com_pre_def
-  Abs_Com_internal_pre_inverse[OF UNIV_I]
-  set1_Com_internal_pre_def set2_Com_internal_pre_def
-  set3_Com_internal_pre_def set4_Com_internal_pre_def
+  Abs_comP_pre_inverse[OF UNIV_I]
+  set1_comP_pre_def set2_comP_pre_def set4_comP_pre_def set3_comP_pre_def
+  Abs_comP_internal_pre_inverse[OF UNIV_I]
+  set1_comP_internal_pre_def set2_comP_internal_pre_def
+  set3_comP_internal_pre_def set4_comP_internal_pre_def
 
-lemma FFVars_Com_simps[simp]:
-  "FFVars_Com (Finp x y t) = {x, y} \<union> FFVars t"
-  "FFVars_Com (Fout x y t) = {x, y} \<union> FFVars t"
-  "FFVars_Com (Binp x y t) = {x} \<union> (FFVars t - {y})"
-  "FFVars_Com (Bout x y t) = {x} \<union> (FFVars t - {y})"
-  "FFVars_Com (Tau t) = FFVars t"
+lemma FFVars_comP_simps[simp]:
+  "FFVars_comP (Finp x y t) = {x, y} \<union> FFVars t"
+  "FFVars_comP (Fout x y t) = {x, y} \<union> FFVars t"
+  "FFVars_comP (Binp x y t) = {x} \<union> (FFVars t - {y})"
+  "FFVars_comP (Bout x y t) = {x} \<union> (FFVars t - {y})"
+  "FFVars_comP (Tau t) = FFVars t"
   apply (unfold Binp_def Bout_def Finp_def Fout_def Tau_def)
-  apply (unfold Com_internal.FFVars_cctors(2))
+  apply (unfold comP_internal.FFVars_cctors(2))
   apply (unfold toUnfold)
-      apply (unfold Com_internal.FFVars_cctors(1))
+      apply (unfold comP_internal.FFVars_cctors(1))
   apply (unfold toUnfold)
   apply auto
   done
 
-lemmas Com_pre.map_id0[simp]
-lemmas Com_pre_map_cong_id = Com_pre.map_cong[of _ _ "id::var\<Rightarrow>var" "id::var\<Rightarrow>var" _ _ _ id _ id, simplified]
+lemmas comP_pre.map_id0[simp]
+lemmas comP_pre_map_cong_id = comP_pre.map_cong[of _ _ "id::var\<Rightarrow>var" "id::var\<Rightarrow>var" _ _ _ id _ id, simplified]
 
-lemma map_Com_pre_Inl_aux: "bij f \<Longrightarrow> |supp f| <o |UNIV::var set| \<Longrightarrow>
- map_Com_pre (id::var\<Rightarrow>var) (f::var\<Rightarrow>var) (rrename_Com_internal f) id (Abs_Com_pre (Inl (x, y, P))) =
- Abs_Com_pre (Inl (x, y, P))"
-apply(rule Com_pre_map_cong_id) unfolding toUnfold by auto
+lemma map_comP_pre_Inl_aux: "bij f \<Longrightarrow> |supp f| <o |UNIV::var set| \<Longrightarrow>
+ map_comP_pre (id::var\<Rightarrow>var) (f::var\<Rightarrow>var) (rrename_comP_internal f) id (Abs_comP_pre (Inl (x, y, P))) =
+ Abs_comP_pre (Inl (x, y, P))"
+apply(rule comP_pre_map_cong_id) unfolding toUnfold by auto
 
-lemma map_Com_pre_Inr_Inl_aux: "bij f \<Longrightarrow> |supp f| <o |UNIV::var set| \<Longrightarrow>
- map_Com_pre (id::var\<Rightarrow>var) (f::var\<Rightarrow>var) (rrename_Com_internal f) id (Abs_Com_pre (Inr (Inl (x, y, P)))) =
- Abs_Com_pre (Inr (Inl (x, y, P)))"
-apply(rule Com_pre_map_cong_id) unfolding toUnfold by auto
+lemma map_comP_pre_Inr_Inl_aux: "bij f \<Longrightarrow> |supp f| <o |UNIV::var set| \<Longrightarrow>
+ map_comP_pre (id::var\<Rightarrow>var) (f::var\<Rightarrow>var) (rrename_comP_internal f) id (Abs_comP_pre (Inr (Inl (x, y, P)))) =
+ Abs_comP_pre (Inr (Inl (x, y, P)))"
+apply(rule comP_pre_map_cong_id) unfolding toUnfold by auto
 
-lemma map_Com_pre_Inr_Inr_Inl_aux: "bij f \<Longrightarrow> |supp f| <o |UNIV::var set| \<Longrightarrow>
- map_Com_pre id f (rrename_Com_internal f) id
-          (Abs_Com_pre (Inr (Inr (Inl (x::var, y::var, Com_internal_ctor (Abs_Com_internal_pre P)))))) =
- Abs_Com_pre (Inr (Inr (Inl (x, f y, Com_internal_ctor (Abs_Com_internal_pre (rrename f P))))))"
-unfolding map_Com_pre_def toUnfold apply auto
-unfolding Com_internal.rrename_cctors(1)
-unfolding map_Com_internal_pre_def by (simp add: toUnfold(27))
+lemma map_comP_pre_Inr_Inr_Inl_aux: "bij f \<Longrightarrow> |supp f| <o |UNIV::var set| \<Longrightarrow>
+ map_comP_pre id f (rrename_comP_internal f) id
+          (Abs_comP_pre (Inr (Inr (Inl (x::var, y::var, comP_internal_ctor (Abs_comP_internal_pre P)))))) =
+ Abs_comP_pre (Inr (Inr (Inl (x, f y, comP_internal_ctor (Abs_comP_internal_pre (rrename f P))))))"
+unfolding map_comP_pre_def toUnfold apply auto
+unfolding comP_internal.rrename_cctors(1)
+unfolding map_comP_internal_pre_def by (simp add: toUnfold(27))
 
-lemma map_Com_pre_Inr_Inr_Inr_Inl_aux: "bij f \<Longrightarrow> |supp f| <o |UNIV::var set| \<Longrightarrow>
- map_Com_pre (id::var\<Rightarrow>var) (f::var\<Rightarrow>var) (rrename_Com_internal f) id (Abs_Com_pre (Inr (Inr (Inr (Inl P))))) =
- Abs_Com_pre (Inr (Inr (Inr (Inl P))))"
-apply(rule Com_pre_map_cong_id) unfolding toUnfold by auto
+lemma map_comP_pre_Inr_Inr_Inr_Inl_aux: "bij f \<Longrightarrow> |supp f| <o |UNIV::var set| \<Longrightarrow>
+ map_comP_pre (id::var\<Rightarrow>var) (f::var\<Rightarrow>var) (rrename_comP_internal f) id (Abs_comP_pre (Inr (Inr (Inr (Inl P))))) =
+ Abs_comP_pre (Inr (Inr (Inr (Inl P))))"
+apply(rule comP_pre_map_cong_id) unfolding toUnfold by auto
 
-lemma map_Com_pre_Inr_Inr_Inr_Inr_aux: "bij f \<Longrightarrow> |supp f| <o |UNIV::var set| \<Longrightarrow>
- map_Com_pre (id::var\<Rightarrow>var) (f::var\<Rightarrow>var) (rrename_Com_internal f) id (Abs_Com_pre (Inr (Inr (Inr (Inr (x::var, y::var, Com_internal_ctor (Abs_Com_internal_pre P))))))) =
- Abs_Com_pre (Inr (Inr (Inr (Inr (x, f y, Com_internal_ctor (Abs_Com_internal_pre (rrename f P)))))))"
-unfolding map_Com_pre_def toUnfold apply auto
-unfolding Com_internal.rrename_cctors(1)
-unfolding map_Com_internal_pre_def by (simp add: toUnfold(27))
+lemma map_comP_pre_Inr_Inr_Inr_Inr_aux: "bij f \<Longrightarrow> |supp f| <o |UNIV::var set| \<Longrightarrow>
+ map_comP_pre (id::var\<Rightarrow>var) (f::var\<Rightarrow>var) (rrename_comP_internal f) id (Abs_comP_pre (Inr (Inr (Inr (Inr (x::var, y::var, comP_internal_ctor (Abs_comP_internal_pre P))))))) =
+ Abs_comP_pre (Inr (Inr (Inr (Inr (x, f y, comP_internal_ctor (Abs_comP_internal_pre (rrename f P)))))))"
+unfolding map_comP_pre_def toUnfold apply auto
+unfolding comP_internal.rrename_cctors(1)
+unfolding map_comP_internal_pre_def by (simp add: toUnfold(27))
 
-lemma Abs_Com_pre_inj[simp]: "Abs_Com_pre k = Abs_Com_pre k' \<longleftrightarrow> k = k'"
+lemma Abs_comP_pre_inj[simp]: "Abs_comP_pre k = Abs_comP_pre k' \<longleftrightarrow> k = k'"
 by (metis toUnfold(22))
 
-lemma Abs_Com_internal_pre_inj[simp]: "Abs_Com_internal_pre k = Abs_Com_internal_pre k' \<longleftrightarrow> k = k'"
+lemma Abs_comP_internal_pre_inj[simp]: "Abs_comP_internal_pre k = Abs_comP_internal_pre k' \<longleftrightarrow> k = k'"
 by (metis toUnfold(27))
 
 lemma Finp_inj[simp]: "Finp x y P = Finp x' y' P' \<longleftrightarrow> x = x' \<and> y = y' \<and> P = P'"
-unfolding Finp_def unfolding Com_internal.TT_injects0 apply simp
+unfolding Finp_def unfolding comP_internal.TT_injects0 apply simp
 unfolding toUnfold apply auto
-  subgoal for f apply(subst (asm) map_Com_pre_Inl_aux) by auto
-  subgoal for f apply(subst (asm) map_Com_pre_Inl_aux) by auto
-  subgoal for f apply(subst (asm) map_Com_pre_Inl_aux) by auto
-  subgoal apply(rule exI[of _ id]) apply(subst map_Com_pre_Inl_aux) by auto .
+  subgoal for f apply(subst (asm) map_comP_pre_Inl_aux) by auto
+  subgoal for f apply(subst (asm) map_comP_pre_Inl_aux) by auto
+  subgoal for f apply(subst (asm) map_comP_pre_Inl_aux) by auto
+  subgoal apply(rule exI[of _ id]) apply(subst map_comP_pre_Inl_aux) by auto .
 
 lemma Fout_inj[simp]: "Fout x y P = Fout x' y' P' \<longleftrightarrow> x = x' \<and> y = y' \<and> P = P'"
-unfolding Fout_def unfolding Com_internal.TT_injects0 apply simp
+unfolding Fout_def unfolding comP_internal.TT_injects0 apply simp
 unfolding toUnfold apply auto
-  subgoal for f apply(subst (asm) map_Com_pre_Inr_Inl_aux) by auto
-  subgoal for f apply(subst (asm) map_Com_pre_Inr_Inl_aux) by auto
-  subgoal for f apply(subst (asm) map_Com_pre_Inr_Inl_aux) by auto
-  subgoal apply(rule exI[of _ id]) apply(subst map_Com_pre_Inr_Inl_aux) by auto .
+  subgoal for f apply(subst (asm) map_comP_pre_Inr_Inl_aux) by auto
+  subgoal for f apply(subst (asm) map_comP_pre_Inr_Inl_aux) by auto
+  subgoal for f apply(subst (asm) map_comP_pre_Inr_Inl_aux) by auto
+  subgoal apply(rule exI[of _ id]) apply(subst map_comP_pre_Inr_Inl_aux) by auto .
 
 lemma Bout_inj[simp]: "Bout x y P = Bout x' y' P' \<longleftrightarrow> x = x' \<and> ((y' \<notin> FFVars P \<or> y' = y) \<and> P' = swap P y y')"
-unfolding Bout_def unfolding Com_internal.TT_injects0 apply simp
+unfolding Bout_def unfolding comP_internal.TT_injects0 apply simp
 unfolding toUnfold apply auto
-  subgoal for f apply(subst (asm) map_Com_pre_Inr_Inr_Inl_aux) by auto
-  subgoal for f apply(subst (asm) map_Com_pre_Inr_Inr_Inl_aux)
-  unfolding id_on_def apply auto unfolding Com_internal.FFVars_cctors(1) toUnfold by auto
-  subgoal for f apply(subst (asm) map_Com_pre_Inr_Inr_Inl_aux)
-  unfolding id_on_def apply auto unfolding Com_internal.FFVars_cctors(1) toUnfold
-  unfolding Com_internal.TT_injects0(1) id_on_def
-  unfolding map_Com_internal_pre_def apply (auto simp: toUnfold id_on_def)
+  subgoal for f apply(subst (asm) map_comP_pre_Inr_Inr_Inl_aux) by auto
+  subgoal for f apply(subst (asm) map_comP_pre_Inr_Inr_Inl_aux)
+  unfolding id_on_def apply auto unfolding comP_internal.FFVars_cctors(1) toUnfold by auto
+  subgoal for f apply(subst (asm) map_comP_pre_Inr_Inr_Inl_aux)
+  unfolding id_on_def apply auto unfolding comP_internal.FFVars_cctors(1) toUnfold
+  unfolding comP_internal.TT_injects0(1) id_on_def
+  unfolding map_comP_internal_pre_def apply (auto simp: toUnfold id_on_def)
   apply(rule rrename_cong) by auto
   subgoal apply(rule exI[of _ "(id(y:=y',y':=y))"])
-  apply(subst map_Com_pre_Inr_Inr_Inl_aux) apply auto
-  unfolding Com_internal.FFVars_cctors(1) by (auto simp: toUnfold id_on_def)
+  apply(subst map_comP_pre_Inr_Inr_Inl_aux) apply auto
+  unfolding comP_internal.FFVars_cctors(1) by (auto simp: toUnfold id_on_def)
   subgoal apply(rule exI[of _ "(id(y:=y',y':=y))"])
-  apply(subst map_Com_pre_Inr_Inr_Inl_aux) by auto .
+  apply(subst map_comP_pre_Inr_Inr_Inl_aux) by auto .
 
 lemma Binp_inj[simp]: "Binp x y P = Binp x' y' P' \<longleftrightarrow> x = x' \<and> ((y' \<notin> FFVars P \<or> y' = y) \<and> P' = swap P y y')"
-unfolding Binp_def unfolding Com_internal.TT_injects0 apply simp
+unfolding Binp_def unfolding comP_internal.TT_injects0 apply simp
 unfolding toUnfold apply auto
-  subgoal for f apply(subst (asm) map_Com_pre_Inr_Inr_Inr_Inr_aux) by auto
-  subgoal for f apply(subst (asm) map_Com_pre_Inr_Inr_Inr_Inr_aux)
-  unfolding id_on_def apply auto unfolding Com_internal.FFVars_cctors(1) toUnfold by auto
-  subgoal for f apply(subst (asm) map_Com_pre_Inr_Inr_Inr_Inr_aux)
-  unfolding id_on_def apply auto unfolding Com_internal.FFVars_cctors(1) toUnfold
-  unfolding Com_internal.TT_injects0(1) id_on_def
-  unfolding map_Com_internal_pre_def apply (auto simp: toUnfold id_on_def)
+  subgoal for f apply(subst (asm) map_comP_pre_Inr_Inr_Inr_Inr_aux) by auto
+  subgoal for f apply(subst (asm) map_comP_pre_Inr_Inr_Inr_Inr_aux)
+  unfolding id_on_def apply auto unfolding comP_internal.FFVars_cctors(1) toUnfold by auto
+  subgoal for f apply(subst (asm) map_comP_pre_Inr_Inr_Inr_Inr_aux)
+  unfolding id_on_def apply auto unfolding comP_internal.FFVars_cctors(1) toUnfold
+  unfolding comP_internal.TT_injects0(1) id_on_def
+  unfolding map_comP_internal_pre_def apply (auto simp: toUnfold id_on_def)
   apply(rule rrename_cong) by auto
   subgoal apply(rule exI[of _ "(id(y:=y',y':=y))"])
-  apply(subst map_Com_pre_Inr_Inr_Inr_Inr_aux) apply auto
-  unfolding Com_internal.FFVars_cctors(1) by (auto simp: toUnfold id_on_def)
+  apply(subst map_comP_pre_Inr_Inr_Inr_Inr_aux) apply auto
+  unfolding comP_internal.FFVars_cctors(1) by (auto simp: toUnfold id_on_def)
   subgoal apply(rule exI[of _ "(id(y:=y',y':=y))"])
-  apply(subst map_Com_pre_Inr_Inr_Inr_Inr_aux) by auto .
+  apply(subst map_comP_pre_Inr_Inr_Inr_Inr_aux) by auto .
 
 lemma Tau_inj[simp]: "Tau P = Tau P' \<longleftrightarrow> P = P'"
-unfolding Tau_def unfolding Com_internal.TT_injects0 apply simp
+unfolding Tau_def unfolding comP_internal.TT_injects0 apply simp
 unfolding toUnfold apply auto
-  subgoal for f apply(subst (asm) map_Com_pre_Inr_Inr_Inr_Inl_aux) by auto
-  subgoal apply(rule exI[of _ id]) apply(subst map_Com_pre_Inr_Inr_Inr_Inl_aux) by auto .
+  subgoal for f apply(subst (asm) map_comP_pre_Inr_Inr_Inr_Inl_aux) by auto
+  subgoal apply(rule exI[of _ id]) apply(subst map_comP_pre_Inr_Inr_Inr_Inl_aux) by auto .
 
 (* *)
 
 lemma Finp_Fout_diff[simp]: "Finp x y P \<noteq> Fout x' y' P'"
 unfolding Finp_def Fout_def
-by (metis Abs_Com_pre_inj Inl_Inr_False Com_internal.TT_injects0(2) map_Com_pre_Inl_aux)
+by (metis Abs_comP_pre_inj Inl_Inr_False comP_internal.TT_injects0(2) map_comP_pre_Inl_aux)
 
 lemmas Fout_Finp_diff[simp] = Finp_Fout_diff[symmetric]
 
 lemma Finp_Bout_diff[simp]: "Finp x y P \<noteq> Bout x' y' P'"
 unfolding Finp_def Bout_def
-by (metis Abs_Com_pre_inj Inl_Inr_False Com_internal.TT_injects0(2) map_Com_pre_Inl_aux)
+by (metis Abs_comP_pre_inj Inl_Inr_False comP_internal.TT_injects0(2) map_comP_pre_Inl_aux)
 
 lemmas Bout_Finp_diff[simp] = Finp_Bout_diff[symmetric]
 
 lemma Finp_Tau_diff[simp]: "Finp x y P \<noteq> Tau P'"
 unfolding Finp_def Tau_def
-by (metis Abs_Com_pre_inj Inl_Inr_False Com_internal.TT_injects0(2) map_Com_pre_Inl_aux)
+by (metis Abs_comP_pre_inj Inl_Inr_False comP_internal.TT_injects0(2) map_comP_pre_Inl_aux)
 
 lemmas Tau_Finp_diff[simp] = Finp_Tau_diff[symmetric]
 
 lemma Fout_Bout_diff[simp]: "Fout x y P \<noteq> Bout x' y' P'"
 unfolding Fout_def Bout_def
-by (metis Abs_Com_pre_inj Inl_Inr_False Com_internal.TT_injects0(2) map_Com_pre_Inr_Inl_aux sum.inject(2))
+by (metis Abs_comP_pre_inj Inl_Inr_False comP_internal.TT_injects0(2) map_comP_pre_Inr_Inl_aux sum.inject(2))
 
 lemmas Bout_Fout_diff[simp] = Fout_Bout_diff[symmetric]
 
 lemma Fout_Tau_diff[simp]: "Fout x y P \<noteq> Tau P'"
 unfolding Fout_def Tau_def
-by (metis Abs_Com_pre_inj Inl_Inr_False Com_internal.TT_injects0(2) map_Com_pre_Inr_Inl_aux sum.inject(2))
+by (metis Abs_comP_pre_inj Inl_Inr_False comP_internal.TT_injects0(2) map_comP_pre_Inr_Inl_aux sum.inject(2))
 
 lemmas Tau_Fout_diff[simp] = Fout_Tau_diff[symmetric]
 
 lemma Bout_Tau_diff[simp]: "Bout x y P \<noteq> Tau P'"
 unfolding Bout_def Tau_def
-by (smt (verit) Inl_Inr_False Inr_inject Com_internal.TT_injects0(2) map_Com_pre_Inr_Inr_Inl_aux toUnfold(22))
+by (smt (verit) Inl_Inr_False Inr_inject comP_internal.TT_injects0(2) map_comP_pre_Inr_Inr_Inl_aux toUnfold(22))
 
 lemmas Tau_Bout_diff[simp] = Bout_Tau_diff[symmetric]
 
 lemma Binp_Bout_diff[simp]: "Binp x y P \<noteq> Bout x' y' P'"
   unfolding Binp_def Bout_def
-  by (smt (verit) Inl_Inr_False Inr_inject Com_internal.TT_injects0(2) map_Com_pre_Inr_Inr_Inl_aux toUnfold(22))
+  by (smt (verit) Inl_Inr_False Inr_inject comP_internal.TT_injects0(2) map_comP_pre_Inr_Inr_Inl_aux toUnfold(22))
 
 lemmas Bout_Binp_diff[simp] = Binp_Bout_diff[symmetric]
 
 lemma Binp_Finp_diff[simp]: "Binp x y P \<noteq> Finp x' y' P'"
   unfolding Binp_def Finp_def
-  by (metis Abs_Com_pre_inj Inl_Inr_False Com_internal.TT_injects0(2) map_Com_pre_Inl_aux)
+  by (metis Abs_comP_pre_inj Inl_Inr_False comP_internal.TT_injects0(2) map_comP_pre_Inl_aux)
 
 lemmas Finp_Binp_diff[simp] = Binp_Finp_diff[symmetric]
 
 lemma Binp_Fout_diff[simp]: "Binp x y P \<noteq> Fout x' y' P'"
   unfolding Binp_def Fout_def
-  by (metis Abs_Com_pre_inj Inl_Inr_False Inr_inject Com_internal.TT_injects0(2) map_Com_pre_Inr_Inl_aux)
+  by (metis Abs_comP_pre_inj Inl_Inr_False Inr_inject comP_internal.TT_injects0(2) map_comP_pre_Inr_Inl_aux)
 
 lemmas Fout_Binp_diff[simp] = Binp_Fout_diff[symmetric]
 
 lemma Binp_Tau_diff[simp]: "Binp x y P \<noteq> Tau P'"
   unfolding Binp_def Tau_def
-  by (metis Abs_Com_pre_inj Inr_not_Inl Com_internal.TT_injects0(2) map_Com_pre_Inr_Inr_Inr_Inl_aux old.sum.inject(2))
+  by (metis Abs_comP_pre_inj Inr_not_Inl comP_internal.TT_injects0(2) map_comP_pre_Inr_Inr_Inr_Inl_aux old.sum.inject(2))
 
 lemmas Tau_Binp_diff[simp] = Binp_Tau_diff[symmetric]
 
 (* Supply of fresh variables *)
 
-lemma finite_FFVars_Com: "finite (FFVars_Com C)"
+lemma finite_FFVars_comP: "finite (FFVars_comP C)"
 unfolding ls_UNIV_iff_finite[symmetric]
-by (simp add: Com_internal.card_of_FFVars_bounds(2))
+by (simp add: comP_internal.card_of_FFVars_bounds(2))
 
 lemma exists_fresh:
-"\<exists> z. z \<notin> set xs \<and> (\<forall>P \<in> set Cs. z \<notin> FFVars_Com P)"
+"\<exists> z. z \<notin> set xs \<and> (\<forall>P \<in> set Cs. z \<notin> FFVars_comP P)"
 proof-
-  have 0: "|set xs \<union> \<Union> (FFVars_Com ` (set Cs))| <o |UNIV::var set|"
+  have 0: "|set xs \<union> \<Union> (FFVars_comP ` (set Cs))| <o |UNIV::var set|"
   unfolding ls_UNIV_iff_finite
-  using finite_FFVars_Com by blast
-  then obtain x where "x \<notin> set xs \<union> \<Union> (FFVars_Com ` (set Cs))"
+  using finite_FFVars_comP by blast
+  then obtain x where "x \<notin> set xs \<union> \<Union> (FFVars_comP ` (set Cs))"
   by (meson ex_new_if_finite finite_iff_le_card_var
-    infinite_iff_natLeq_ordLeq var_Proc_pre_class.large)
+    infinite_iff_natLeq_ordLeq var_procP_pre_class.large)
   thus ?thesis by auto
 qed
 
 (* *)
 
-lemma rrename_Com_Finp[simp]: "bij \<sigma> \<Longrightarrow> |supp \<sigma>| <o |UNIV::var set| \<Longrightarrow>
-  rrename_Com \<sigma> (Finp a u P) = Finp (\<sigma> a) (\<sigma> u) (rrename \<sigma> P)"
-unfolding Finp_def unfolding Com_internal.rrename_cctors
-unfolding map_Com_pre_def unfolding toUnfold by simp
+lemma rrename_comP_Finp[simp]: "bij \<sigma> \<Longrightarrow> |supp \<sigma>| <o |UNIV::var set| \<Longrightarrow>
+  rrename_comP \<sigma> (Finp a u P) = Finp (\<sigma> a) (\<sigma> u) (rrename \<sigma> P)"
+unfolding Finp_def unfolding comP_internal.rrename_cctors
+unfolding map_comP_pre_def unfolding toUnfold by simp
 
-lemma rrename_Com_Fout[simp]: "bij \<sigma> \<Longrightarrow> |supp \<sigma>| <o |UNIV::var set| \<Longrightarrow>
-  rrename_Com \<sigma> (Fout a u P) = Fout (\<sigma> a) (\<sigma> u) (rrename \<sigma> P)"
-unfolding Fout_def unfolding Com_internal.rrename_cctors
-unfolding map_Com_pre_def unfolding toUnfold by simp
+lemma rrename_comP_Fout[simp]: "bij \<sigma> \<Longrightarrow> |supp \<sigma>| <o |UNIV::var set| \<Longrightarrow>
+  rrename_comP \<sigma> (Fout a u P) = Fout (\<sigma> a) (\<sigma> u) (rrename \<sigma> P)"
+unfolding Fout_def unfolding comP_internal.rrename_cctors
+unfolding map_comP_pre_def unfolding toUnfold by simp
 
-lemma rrename_Com_Bout[simp]: "bij \<sigma> \<Longrightarrow> |supp \<sigma>| <o |UNIV::var set| \<Longrightarrow>
-  rrename_Com \<sigma> (Bout a u P) = Bout (\<sigma> a) (\<sigma> u) (rrename \<sigma> P)"
-unfolding Bout_def unfolding Com_internal.rrename_cctors
-unfolding map_Com_pre_def unfolding toUnfold
-unfolding Com_internal.rrename_cctors(1)
-unfolding map_Com_internal_pre_def unfolding toUnfold by simp
+lemma rrename_comP_Bout[simp]: "bij \<sigma> \<Longrightarrow> |supp \<sigma>| <o |UNIV::var set| \<Longrightarrow>
+  rrename_comP \<sigma> (Bout a u P) = Bout (\<sigma> a) (\<sigma> u) (rrename \<sigma> P)"
+unfolding Bout_def unfolding comP_internal.rrename_cctors
+unfolding map_comP_pre_def unfolding toUnfold
+unfolding comP_internal.rrename_cctors(1)
+unfolding map_comP_internal_pre_def unfolding toUnfold by simp
 
-lemma rrename_Com_Binp[simp]: "bij \<sigma> \<Longrightarrow> |supp \<sigma>| <o |UNIV::var set| \<Longrightarrow>
-  rrename_Com \<sigma> (Binp a u P) = Binp (\<sigma> a) (\<sigma> u) (rrename \<sigma> P)"
-unfolding Binp_def unfolding Com_internal.rrename_cctors
-unfolding map_Com_pre_def unfolding toUnfold
-unfolding Com_internal.rrename_cctors(1)
-unfolding map_Com_internal_pre_def unfolding toUnfold by simp
+lemma rrename_comP_Binp[simp]: "bij \<sigma> \<Longrightarrow> |supp \<sigma>| <o |UNIV::var set| \<Longrightarrow>
+  rrename_comP \<sigma> (Binp a u P) = Binp (\<sigma> a) (\<sigma> u) (rrename \<sigma> P)"
+unfolding Binp_def unfolding comP_internal.rrename_cctors
+unfolding map_comP_pre_def unfolding toUnfold
+unfolding comP_internal.rrename_cctors(1)
+unfolding map_comP_internal_pre_def unfolding toUnfold by simp
 
-lemma rrename_Com_Tau[simp]: "bij \<sigma> \<Longrightarrow> |supp \<sigma>| <o |UNIV::var set| \<Longrightarrow>
-  rrename_Com \<sigma> (Tau P) = Tau (rrename \<sigma> P)"
-unfolding Tau_def unfolding Com_internal.rrename_cctors
-unfolding map_Com_pre_def unfolding toUnfold
-unfolding Com_internal.rrename_cctors(1)
-unfolding map_Com_internal_pre_def unfolding toUnfold by simp
+lemma rrename_comP_Tau[simp]: "bij \<sigma> \<Longrightarrow> |supp \<sigma>| <o |UNIV::var set| \<Longrightarrow>
+  rrename_comP \<sigma> (Tau P) = Tau (rrename \<sigma> P)"
+unfolding Tau_def unfolding comP_internal.rrename_cctors
+unfolding map_comP_pre_def unfolding toUnfold
+unfolding comP_internal.rrename_cctors(1)
+unfolding map_comP_internal_pre_def unfolding toUnfold by simp
 
 (* Actions *)
 
@@ -338,10 +338,10 @@ fun ns :: "act \<Rightarrow> var set" where
 abbreviation "bvars \<equiv> bns"
 abbreviation "fvars \<equiv> fns"
 
-lemma bns_bound: "|bns \<alpha>| <o |UNIV::'a::var_Com_pre set|"
-  by (metis Commitment.var_ID_class.large bns.elims finite_iff_le_card_var finite_ordLess_infinite2 insert_bound large_imp_infinite singl_bound)
+lemma bns_bound: "|bns \<alpha>| <o |UNIV::'a::var_comP_pre set|"
+  by (metis var_ID_class.large bns.elims finite_iff_le_card_var finite_ordLess_infinite2 insert_bound large_imp_infinite singl_bound)
 
-local_setup \<open>MRBNF_Sugar.register_binder_sugar "Commitment.Com" {
+local_setup \<open>MRBNF_Sugar.register_binder_sugar "Commitment.comP" {
   ctors = [
     (@{term Finp}, @{thm Finp_def}),
     (@{term Fout}, @{thm Fout_def}),
@@ -362,7 +362,7 @@ local_setup \<open>MRBNF_Sugar.register_binder_sugar "Commitment.Com" {
   ]],
   bset_bounds = @{thms bns_bound},
   strong_induct = @{thm refl},
-  mrbnf = the (MRBNF_Def.mrbnf_of @{context} "Commitment.Com_pre"),
+  mrbnf = the (MRBNF_Def.mrbnf_of @{context} "Commitment.comP_pre"),
   set_simpss = [],
   subst_simps = NONE
 }\<close>
@@ -372,9 +372,9 @@ abbreviation "swapa act x y \<equiv> map_action (id(x:=y,y:=x)) act"
 lemma bvars_map_action[simp]: "bvars (map_action \<sigma> act) = image \<sigma> (bvars act)"
 by (cases act, auto)
 
-lemma rrename_Com_Cmt[simp]:
+lemma rrename_comP_Cmt[simp]:
 "bij \<sigma> \<and> |supp \<sigma>| <o |UNIV::var set| \<Longrightarrow>
- rrename_Com \<sigma> (Cmt act P) = Cmt (map_action \<sigma> act) (rrename \<sigma> P)"
+ rrename_comP \<sigma> (Cmt act P) = Cmt (map_action \<sigma> act) (rrename \<sigma> P)"
 by (cases act, auto)
 
 lemma bvars_act_bout: "bvars act = {} \<or> (\<exists>a b. act = bout a b) \<or> (\<exists>a b. act = binp a b)"
