thys/Infinitary_FOL/InfFOL.thy
@@ -1,4 +1,4 @@
-theory InfFOL imports InfFmla 
+theory InfFOL imports InfFmla
 begin
 
 binder_inductive deduct :: "fmla set\<^sub>k \<Rightarrow> fmla \<Rightarrow> bool" (infix "\<turnstile>" 100) where
@@ -7,44 +7,44 @@ binder_inductive deduct :: "fmla set\<^sub>k \<Rightarrow> fmla \<Rightarrow> bo
 | ConjE: "\<lbrakk> \<Delta> \<turnstile> Conj F ; f \<in>\<^sub>k\<^sub>1 F \<rbrakk> \<Longrightarrow> \<Delta> \<turnstile> f"
 | NegI: "\<Delta>,f \<turnstile> \<bottom> \<Longrightarrow> \<Delta> \<turnstile> Neg f"
 | NegE: "\<lbrakk> \<Delta> \<turnstile> Neg f ; \<Delta> \<turnstile> f \<rbrakk> \<Longrightarrow> \<Delta> \<turnstile> \<bottom>"
-| AllI: "\<lbrakk> \<Delta> \<turnstile> f ; set\<^sub>k\<^sub>2 V \<inter> \<Union>(FFVars_Fmla ` set\<^sub>k \<Delta>) = {} \<rbrakk> \<Longrightarrow> \<Delta> \<turnstile> All V f"
+| AllI: "\<lbrakk> \<Delta> \<turnstile> f ; set\<^sub>k\<^sub>2 V \<inter> \<Union>(FFVars_fmlaP ` set\<^sub>k \<Delta>) = {} \<rbrakk> \<Longrightarrow> \<Delta> \<turnstile> All V f"
 | AllE: "\<lbrakk> \<Delta> \<turnstile> All V f ; supp \<rho> \<subseteq> set\<^sub>k\<^sub>2 V \<rbrakk> \<Longrightarrow> \<Delta> \<turnstile> f\<lbrakk>\<rho>\<rbrakk>"
   subgoal for R B \<sigma> x1 x2
     unfolding induct_rulify_fallback split_beta
     apply (elim disj_forward exE)
-          apply (auto simp: Fmla.rrename_comps in_k_equiv in_k_equiv' isPerm_def Fmla.rrename_ids supp_inv_bound)
+          apply (auto simp: fmlaP.rrename_comps in_k_equiv in_k_equiv' isPerm_def fmlaP.rrename_ids supp_inv_bound)
          apply (rule exI)
          apply (rule conjI)
           apply (rule refl)
          apply (rule allI impI)+
          apply (unfold set\<^sub>k.map_comp)
-         apply (subst Fmla.rrename_comp0s)
+         apply (subst fmlaP.rrename_comp0s)
              apply (assumption | rule bij_imp_bij_inv supp_inv_bound)+
          apply (subst inv_o_simp1, assumption)
-         apply (unfold Fmla.rrename_id0s set\<^sub>k.map_id)
+         apply (unfold fmlaP.rrename_id0s set\<^sub>k.map_id)
          apply (rotate_tac -1)
          apply (drule iffD2[OF in_k1_equiv, of "inv \<sigma>", rotated])
           apply (unfold isPerm_def)
           apply (assumption | rule conjI bij_imp_bij_inv supp_inv_bound)+
          apply (subst (asm) set\<^sub>k\<^sub>1.map_comp)
-         apply (subst (asm) Fmla.rrename_comp0s)
+         apply (subst (asm) fmlaP.rrename_comp0s)
              apply (assumption | rule bij_imp_bij_inv supp_inv_bound)+
          apply (subst (asm) inv_o_simp1, assumption)
-         apply (unfold Fmla.rrename_id0s set\<^sub>k\<^sub>1.map_id)
+         apply (unfold fmlaP.rrename_id0s set\<^sub>k\<^sub>1.map_id)
          apply (erule allE)
          apply (erule impE)
           apply assumption+
-        apply (subst Fmla.rrename_comp0s)
+        apply (subst fmlaP.rrename_comp0s)
             apply (assumption | rule bij_imp_bij_inv supp_inv_bound)+
         apply (subst inv_o_simp1, assumption)
-        apply (unfold Fmla.rrename_id0s set\<^sub>k.map_id)
-        apply (metis bij_imp_bij_inv Fmla.rrename_comps Fmla.rrename_ids Fmla_rrename_simps(3) in_k1_equiv' inv_o_simp1 supp_inv_bound)
-       apply (metis Fmla.rrename_bijs Fmla.rrename_inv_simps inv_o_simp1 inv_simp1 set\<^sub>k.map_id)
-      apply (metis Fmla.rrename_bijs Fmla.rrename_inv_simps inv_o_simp1 inv_simp1 set\<^sub>k.map_id)
+        apply (unfold fmlaP.rrename_id0s set\<^sub>k.map_id)
+        apply (metis bij_imp_bij_inv fmlaP.rrename_comps fmlaP.rrename_ids fmlaP_rrename_simps(3) in_k1_equiv' inv_o_simp1 supp_inv_bound)
+       apply (metis fmlaP.rrename_bijs fmlaP.rrename_inv_simps inv_o_simp1 inv_simp1 set\<^sub>k.map_id)
+      apply (metis fmlaP.rrename_bijs fmlaP.rrename_inv_simps inv_o_simp1 inv_simp1 set\<^sub>k.map_id)
     subgoal for f V
-      apply (rule exI[of _ "rrename_Fmla \<sigma> f"])
+      apply (rule exI[of _ "rrename_fmlaP \<sigma> f"])
       apply (rule exI[of _ "map_set\<^sub>k\<^sub>2 \<sigma> V"])
-      by (smt (verit, ccfv_threshold) bij_imp_bij_inv Fmla.rrename_comp0s Fmla.rrename_id0s Fmla.rrename_ids Fmla.set_map0 Fmla_vvsubst_rrename image_Int_empty image_Union image_comp inv_o_simp1 pointfree_idE set\<^sub>k.map_ident_strong set\<^sub>k.set_map set\<^sub>k\<^sub>2.set_map supp_inv_bound)
+      by (smt (verit, ccfv_threshold) bij_imp_bij_inv fmlaP.rrename_comp0s fmlaP.rrename_id0s fmlaP.rrename_ids fmlaP.set_map0 fmlaP_vvsubst_rrename image_Int_empty image_Union image_comp inv_o_simp1 pointfree_idE set\<^sub>k.map_ident_strong set\<^sub>k.set_map set\<^sub>k\<^sub>2.set_map supp_inv_bound)
     subgoal for V f \<rho>
       apply (rule exI[of _ "map_set\<^sub>k\<^sub>2 \<sigma> V"])
       apply (unfold set\<^sub>k\<^sub>2.set_map)
@@ -53,32 +53,32 @@ binder_inductive deduct :: "fmla set\<^sub>k \<Rightarrow> fmla \<Rightarrow> bo
       apply (unfold set\<^sub>k\<^sub>2.map_comp)
       apply (subst inv_o_simp1, assumption)
       apply (unfold set\<^sub>k\<^sub>2.map_id)
-      apply (rule exI[of _ "rrename_Fmla \<sigma> f"])
-      apply (subst Fmla.rrename_comps)
+      apply (rule exI[of _ "rrename_fmlaP \<sigma> f"])
+      apply (subst fmlaP.rrename_comps)
           apply (assumption | rule bij_imp_bij_inv supp_inv_bound)+
       apply (subst inv_o_simp1, assumption)
-      apply (unfold Fmla.rrename_ids)
+      apply (unfold fmlaP.rrename_ids)
       apply (rule exI[of _ "\<sigma> \<circ> \<rho> \<circ> inv \<sigma>"])
       apply (subgoal_tac "|supp \<rho>| <o |UNIV::k set|")
        prefer 2
        apply (erule card_of_subset_bound)
       apply (simp add: small_set\<^sub>k\<^sub>2[unfolded small_def])
-      apply (subst Fmla.map_comp0)
+      apply (subst fmlaP.map_comp0)
         apply (rule supp_inv_bound supp_comp_bound infinite_UNIV | assumption)+
-      apply (subst Fmla.map_comp0)
+      apply (subst fmlaP.map_comp0)
         apply (rule supp_inv_bound supp_comp_bound infinite_UNIV | assumption)+
       apply (subst supp_o_bij)
        apply assumption
       apply (subst comp_apply)
-      apply (unfold Fmla_vvsubst_rrename Fmla_vvsubst_rrename[OF bij_imp_bij_inv supp_inv_bound])
-      apply (subst Fmla.rrename_comps)
+      apply (unfold fmlaP_vvsubst_rrename fmlaP_vvsubst_rrename[OF bij_imp_bij_inv supp_inv_bound])
+      apply (subst fmlaP.rrename_comps)
           apply (rule supp_inv_bound bij_imp_bij_inv | assumption)+
       apply (subst inv_o_simp1, assumption)
-      apply (unfold Fmla.rrename_ids comp_def)
+      apply (unfold fmlaP.rrename_ids comp_def)
       apply (rule conjI)
        apply (rule refl)
       apply (rule conjI)
-      apply (metis Fmla.rrename_bijs Fmla.rrename_inv_simps inv_simp1 set\<^sub>k.map_ident_strong)
+      apply (metis fmlaP.rrename_bijs fmlaP.rrename_inv_simps inv_simp1 set\<^sub>k.map_ident_strong)
       apply (erule image_mono)
       done
     done
@@ -90,18 +90,18 @@ binder_inductive deduct :: "fmla set\<^sub>k \<Rightarrow> fmla \<Rightarrow> bo
      apply (elim exE conjE)
     apply simp
     subgoal for \<Delta> f V
-      apply (rule exE[OF refresh[of V "\<Union>(FFVars_Fmla ` set\<^sub>k \<Delta>) \<union> FFVars_Fmla (All V f)", unfolded Fmla.set
+      apply (rule exE[OF refresh[of V "\<Union>(FFVars_fmlaP ` set\<^sub>k \<Delta>) \<union> FFVars_fmlaP (All V f)", unfolded fmlaP.set
               Un_Diff Diff_idemp
               ]])
         apply blast
-      apply (metis (no_types, lifting) Fmla.set(4) Fmla.set_bd_UNIV set\<^sub>k.set_bd var_Fmla_pre_class.UN_bound var_Fmla_pre_class.Un_bound)
+      apply (metis (no_types, lifting) fmlaP.set(4) fmlaP.set_bd_UNIV set\<^sub>k.set_bd var_fmlaP_pre_class.UN_bound var_fmlaP_pre_class.Un_bound)
       apply (erule exE conjE)+
       subgoal for g VV
-        apply (rule exI[of _ "map_set\<^sub>k (rrename_Fmla g) \<Delta>"])
+        apply (rule exI[of _ "map_set\<^sub>k (rrename_fmlaP g) \<Delta>"])
         apply (rule exI[of _ "g ` set\<^sub>k\<^sub>2 V"])
         apply (rule conjI[rotated])
          apply (metis set\<^sub>k\<^sub>2.set_map)
-        apply (rule exI[of _ "rrename_Fmla g f"])
+        apply (rule exI[of _ "rrename_fmlaP g f"])
         apply (rule exI[of _ VV])
         apply (rule conjI)
          apply (drule arg_cong[of _ _ set\<^sub>k\<^sub>2])
@@ -115,7 +115,7 @@ binder_inductive deduct :: "fmla set\<^sub>k \<Rightarrow> fmla \<Rightarrow> bo
          apply (rule trans)
           apply (rule id_apply)
          apply (rule sym)
-         apply (rule Fmla.rrename_cong_ids)
+         apply (rule fmlaP.rrename_cong_ids)
            apply assumption+
          apply (erule id_onD)
          apply (rule UnI1)
@@ -128,7 +128,7 @@ binder_inductive deduct :: "fmla set\<^sub>k \<Rightarrow> fmla \<Rightarrow> bo
            apply assumption
           apply (rule conjI | assumption)+
 
-         apply (unfold set\<^sub>k.set_map image_comp[unfolded comp_def] Fmla.FFVars_rrenames
+         apply (unfold set\<^sub>k.set_map image_comp[unfolded comp_def] fmlaP.FFVars_rrenames
             image_UN[symmetric]
             )[1]
          apply hypsubst
@@ -140,15 +140,15 @@ binder_inductive deduct :: "fmla set\<^sub>k \<Rightarrow> fmla \<Rightarrow> bo
          apply assumption
 
         apply (subst All_def)+
-        apply (unfold Fmla.TT_injects0)
+        apply (unfold fmlaP.TT_injects0)
         apply (rule exI[of _ g])
         apply (rule conjI, assumption)+
         apply (rule conjI)
 
-         apply (unfold set3_Fmla_pre_def comp_def Abs_Fmla_pre_inverse[OF UNIV_I]
+         apply (unfold set3_fmlaP_pre_def comp_def Abs_fmlaP_pre_inverse[OF UNIV_I]
             map_sum.simps map_prod_simp sum_set_simps prod_set_simps Un_empty cSup_singleton
-            Un_empty_left Un_empty_right Union_empty UN_single set2_Fmla_pre_def set\<^sub>k\<^sub>2.set_map
-            UN_singleton map_Fmla_pre_def
+            Un_empty_left Un_empty_right Union_empty UN_single set2_fmlaP_pre_def set\<^sub>k\<^sub>2.set_map
+            UN_singleton map_fmlaP_pre_def
             )
          apply (erule id_on_antimono)
          apply (rule Un_upper2)
@@ -160,22 +160,22 @@ binder_inductive deduct :: "fmla set\<^sub>k \<Rightarrow> fmla \<Rightarrow> bo
      apply (elim exE conjE)
     apply simp
     apply hypsubst_thin
-    apply (subst Fmla.set_map)
+    apply (subst fmlaP.set_map)
     apply (meson card_of_subset_bound small_def small_set\<^sub>k\<^sub>2)
     apply (unfold triv_forall_equality)
 
     subgoal premises prems for V f \<rho>
     proof -
       define X where "X \<equiv> set\<^sub>k\<^sub>2 V"
-      let ?O = "\<Union> (FFVars_Fmla ` set\<^sub>k \<Delta>) \<union> \<rho> ` FFVars_Fmla f \<union> imsupp \<rho> \<union> X \<union> (FFVars_Fmla f - set\<^sub>k\<^sub>2 V)"
+      let ?O = "\<Union> (FFVars_fmlaP ` set\<^sub>k \<Delta>) \<union> \<rho> ` FFVars_fmlaP f \<union> imsupp \<rho> \<union> X \<union> (FFVars_fmlaP f - set\<^sub>k\<^sub>2 V)"
       have osmall: "|?O| <o |UNIV::var set|"
-        apply (intro var_Fmla_pre_class.Un_bound)
-        apply (meson Fmla.set_bd_UNIV set\<^sub>k.set_bd var_Fmla_pre_class.UN_bound)
-        using Fmla.set_bd_UNIV small_def small_image apply blast
+        apply (intro var_fmlaP_pre_class.Un_bound)
+        apply (meson fmlaP.set_bd_UNIV set\<^sub>k.set_bd var_fmlaP_pre_class.UN_bound)
+        using fmlaP.set_bd_UNIV small_def small_image apply blast
         unfolding imsupp_def
-        apply (meson card_of_image card_of_subset_bound ordLeq_ordLess_trans prems(3) small_def small_set\<^sub>k\<^sub>2 var_Fmla_pre_class.Un_bound)
+        apply (meson card_of_image card_of_subset_bound ordLeq_ordLess_trans prems(3) small_def small_set\<^sub>k\<^sub>2 var_fmlaP_pre_class.Un_bound)
         using X_def small_def small_set\<^sub>k\<^sub>2 apply blast
-        using card_of_minus_bound Fmla.set_bd_UNIV by blast
+        using card_of_minus_bound fmlaP.set_bd_UNIV by blast
 
       obtain W' g where W': "W' \<inter> ?O = {}" "bij_betw g X W'"
       proof atomize_elim
@@ -206,14 +206,14 @@ binder_inductive deduct :: "fmla set\<^sub>k \<Rightarrow> fmla \<Rightarrow> bo
 
       have "|X \<union> W'| <o |UNIV::var set|" unfolding X_def using W'
         using small_set\<^sub>k\<^sub>2[unfolded small_def]
-        by (metis X_def bij_betw_imp_surj_on small_def small_image var_Fmla_pre_class.Un_bound)
+        by (metis X_def bij_betw_imp_surj_on small_def small_image var_fmlaP_pre_class.Un_bound)
       moreover have "supp \<sigma> \<subseteq> X \<union> W'" using \<sigma>(2) unfolding id_on_def by (meson UnI1 UnI2 \<sigma>_def not_in_supp_alt subsetI)
       ultimately have \<sigma>_small: "|supp \<sigma>| <o |UNIV::var set|" using card_of_subset_bound by blast
 
-      define \<rho>' where "\<rho>' \<equiv> \<lambda>x. if x \<in> \<sigma> ` FFVars_Fmla f then (\<rho> \<circ> \<sigma>) x else x"
+      define \<rho>' where "\<rho>' \<equiv> \<lambda>x. if x \<in> \<sigma> ` FFVars_fmlaP f then (\<rho> \<circ> \<sigma>) x else x"
       have "supp \<rho>' \<subseteq> supp (\<rho> \<circ> \<sigma>)" unfolding \<rho>'_def supp_def by auto
       then have \<rho>'_small: "|supp \<rho>'| <o |UNIV::var set|"
-        by (meson \<sigma>_small card_of_subset_bound Fmla_pre.supp_comp_bound prems(3) small_def small_set\<^sub>k\<^sub>2)
+        by (meson \<sigma>_small card_of_subset_bound fmlaP_pre.supp_comp_bound prems(3) small_def small_set\<^sub>k\<^sub>2)
 
       show ?thesis using prems W'
         apply -
@@ -222,17 +222,17 @@ binder_inductive deduct :: "fmla set\<^sub>k \<Rightarrow> fmla \<Rightarrow> bo
         apply (rule conjI)
          apply (rule exI[of _ "map_set\<^sub>k\<^sub>2 \<sigma> V"])
          apply (rule conjI[rotated])+
-           apply (rule exI[of _ "rrename_Fmla \<sigma> f"])
+           apply (rule exI[of _ "rrename_fmlaP \<sigma> f"])
            apply (rule exI[of _ \<rho>'])
 
            apply (rule conjI)
-            apply (subst Fmla_vvsubst_rrename[symmetric])
+            apply (subst fmlaP_vvsubst_rrename[symmetric])
               apply (rule \<sigma>_bij)
              apply (rule \<sigma>_small)
-            apply (subst Fmla.map_comp)
+            apply (subst fmlaP.map_comp)
               apply (rule \<sigma>_small)
              apply (rule \<rho>'_small)
-            apply (rule Fmla.map_cong)
+            apply (rule fmlaP.map_cong)
                apply (meson card_of_subset_bound small_def small_set\<^sub>k\<^sub>2)
               apply (rule supp_comp_bound)
                 apply (rule \<sigma>_small)
@@ -247,11 +247,11 @@ binder_inductive deduct :: "fmla set\<^sub>k \<Rightarrow> fmla \<Rightarrow> bo
              prefer 2
              apply assumption
             apply (rule sym)
-            apply (unfold All_def Fmla.TT_injects0)[1]
-            apply (unfold set3_Fmla_pre_def comp_def Abs_Fmla_pre_inverse[OF UNIV_I]
+            apply (unfold All_def fmlaP.TT_injects0)[1]
+            apply (unfold set3_fmlaP_pre_def comp_def Abs_fmlaP_pre_inverse[OF UNIV_I]
             map_sum.simps map_prod_simp sum_set_simps prod_set_simps Un_empty cSup_singleton
-            Un_empty_left Un_empty_right Union_empty UN_single set2_Fmla_pre_def set\<^sub>k\<^sub>2.set_map
-            UN_singleton map_Fmla_pre_def
+            Un_empty_left Un_empty_right Union_empty UN_single set2_fmlaP_pre_def set\<^sub>k\<^sub>2.set_map
+            UN_singleton map_fmlaP_pre_def
             )[1]
             apply (rule exI[of _ \<sigma>])
             apply (rule conjI, rule \<sigma>_bij)
@@ -262,7 +262,7 @@ binder_inductive deduct :: "fmla set\<^sub>k \<Rightarrow> fmla \<Rightarrow> bo
             apply (rule refl)
 
            apply (unfold set\<^sub>k\<^sub>2.set_map)
-           apply (subgoal_tac "supp (\<rho> \<circ> \<sigma>) \<inter> \<sigma> ` FFVars_Fmla f \<subseteq> \<sigma> ` set\<^sub>k\<^sub>2 V")
+           apply (subgoal_tac "supp (\<rho> \<circ> \<sigma>) \<inter> \<sigma> ` FFVars_fmlaP f \<subseteq> \<sigma> ` set\<^sub>k\<^sub>2 V")
             apply (smt (verit, best) IntI \<rho>'_def not_in_supp_alt subset_iff)
            apply (unfold supp_def imsupp_def)
         using X_def \<sigma>_def apply auto[1]
