thys/Infinitary_Lambda_Calculus/ILC_affine.thy
@@ -8,7 +8,7 @@ begin
 (* *)
 
 lemma Tvars_dsset: "(FFVars t - dsset xs) \<inter> dsset xs = {}" "|FFVars t - dsset xs| <o |UNIV::ivar set|"
-apply auto using card_of_minus_bound ILterm.set_bd_UNIV by blast
+apply auto using card_of_minus_bound iltermP.set_bd_UNIV by blast
 
 binder_inductive affine  :: "ilterm \<Rightarrow> bool" where
  iVr[simp,intro!]: "affine (iVr x)"
@@ -35,7 +35,7 @@ binder_inductive affine  :: "ilterm \<Rightarrow> bool" where
       subgoal apply(elim exE) subgoal for e xs
         apply(rule exI[of _ "irrename \<sigma> e"])
         apply(rule exI[of _ "dsmap \<sigma> xs"])
-        apply (simp add: ILterm.rrename_comps)
+        apply (simp add: iltermP.rrename_comps)
         done
       done
     done
@@ -44,7 +44,7 @@ binder_inductive affine  :: "ilterm \<Rightarrow> bool" where
       subgoal apply(elim exE) subgoal for e1 es2
         apply(rule exI[of _ "irrename \<sigma> e1"])
         apply(rule exI[of _ "smap (irrename \<sigma>) es2"])
-        apply (fastforce simp add: ILterm.rrename_comps)
+        apply (fastforce simp add: iltermP.rrename_comps)
         done
       done
     done
@@ -104,7 +104,7 @@ assumes "affine (iLm xs e)"
 shows "affine e"
 proof-
   obtain xs' e' where 0: "iLm xs e = iLm xs' e'" and "affine e'"
-  using assms by (smt (verit, del_insts) affine.cases ILterm.distinct(2) ILterm.distinct(4))
+  using assms by (smt (verit, del_insts) affine.cases iltermP.distinct(2) iltermP.distinct(4))
   thus ?thesis using 0 unfolding iLm_inject
   by (metis iLm_inject affine.equiv)
 qed
@@ -123,13 +123,13 @@ and r: "affine (e::ilterm)"
 shows "affine (itvsubst f e)"
 using r proof (binder_induction e avoiding: "IImsupp f" rule: affine.strong_induct)
   case (iLm ea xs)
-  show ?case using iLm apply(subst ILterm.subst)
+  show ?case using iLm apply(subst iltermP.subst)
       subgoal using f by auto
       subgoal by auto
       subgoal apply(rule affine.iLm) by auto .
 next
   case (iAp e1 es2)
-  then show ?case apply(subst ILterm.subst)
+  then show ?case apply(subst iltermP.subst)
       subgoal using f by auto
       subgoal apply(rule affine.iAp) using fv f
       by auto (metis Int_emptyD)+ .
@@ -150,7 +150,7 @@ proof-
   have t: "FFVars t = {}" "affine t" unfolding t_def using x by (auto intro: affine.intros)
 
   have fve: "\<And>e. |FFVars e| <o |UNIV::ivar set|"
-    by (simp add: ILterm.set_bd_UNIV)
+    by (simp add: iltermP.set_bd_UNIV)
 
   have "|\<Union> ((FFVars o f) ` (FFVars e))| \<le>o |Sigma (FFVars e) (FFVars o f)|"
   by (rule card_of_UNION_Sigma)
@@ -190,7 +190,7 @@ shows "affine (itvsubst (imkSubst xs es) e)"
 apply(rule tvsubst_affine)
 using assms apply auto
   apply (simp add: imkSubst_def)
-  by (metis Int_emptyD dtheN imkSubst_def ILterm.set(1) singletonD snth_sset)
+  by (metis Int_emptyD dtheN imkSubst_def iltermP.set(1) singletonD snth_sset)
 
 lemma imkSubst_affine_strong:
 assumes r: "affine e" and
@@ -200,7 +200,7 @@ shows "affine (itvsubst (imkSubst xs es) e)"
 apply(rule tvsubst_affine)
 using assms apply auto
   apply (simp add: imkSubst_def)
-  by (smt (verit, best) IntI disjoint_insert(2) dtheN imkSubst_def in_mono ILterm.set(1)
+  by (smt (verit, best) IntI disjoint_insert(2) dtheN imkSubst_def in_mono iltermP.set(1)
   mk_disjoint_insert singletonD snth_sset)
 
 end
