thys/Pi_Calculus/Pi_Transition_Common.thy
@@ -6,11 +6,11 @@ hide_const inverse_class.inverse_divide trans
 no_notation inverse.inverse_divide (infixl "'/" 70)
 
 abbreviation Tsupp :: "proc \<Rightarrow> com \<Rightarrow> var set" where
-"Tsupp e1 e2 \<equiv> FFVars e1 \<union> FFVars_Com e2"
+"Tsupp e1 e2 \<equiv> FFVars e1 \<union> FFVars_comP e2"
 
 (* Supply of fresh variables: *)
 lemma finite_Tsupp: "finite (Tsupp e1 e2)"
-  by (metis FFVars_Com_simps(5) finite_FFVars_Com finite_Un)
+  by (metis FFVars_comP_simps(5) finite_FFVars_comP finite_Un)
 
 lemma finite_vars: "finite (vars act)"
   by (cases act) auto
@@ -23,7 +23,7 @@ proof-
   using finite_Tsupp finite_vars by blast
   then obtain x where "x \<notin> set xs \<union> Tsupp x1 x2 \<union> \<Union> (vars ` (set as))"
   by (meson ex_new_if_finite finite_iff_le_card_var
-    infinite_iff_natLeq_ordLeq var_Proc_pre_class.large)
+    infinite_iff_natLeq_ordLeq var_procP_pre_class.large)
   thus ?thesis by auto
 qed
 
@@ -33,7 +33,7 @@ ML \<open>fun gen_fresh ctxt xs0 acts0 ts0 = HEADGOAL (Subgoal.FOCUS_PARAMS (fn 
     fun mk zs T = filter (fn t => fastype_of t = T) ps |> append zs |> HOLogic.mk_list T |> Thm.cterm_of ctxt;
     val xs = mk xs0 @{typ var};
     val acts = mk acts0 @{typ "var action"};
-    (*val tss = map (mk ts0) [@{typ "var Proc"}, @{typ "var Com"}];*)
+    (*val tss = map (mk ts0) [@{typ "var procP"}, @{typ "var comP"}];*)
     val thm = infer_instantiate' ctxt ([SOME xs, SOME acts] @ map (SOME o Thm.cterm_of ctxt) ts0) @{thm exists_fresh'} RS exE;
   in HEADGOAL (resolve_tac ctxt [thm]) end) ctxt)\<close>
 
@@ -43,7 +43,7 @@ lemma isPerm_swap: "isPerm (id(x := y, y := x))"
 lemma R_forw_subst: "R x y \<Longrightarrow> (\<And>x y. R x y \<Longrightarrow> R (f x) (g y)) \<Longrightarrow> z = g y \<Longrightarrow> R (f x) z"
   by blast
 
-lemma FFVars_Com_Cmt: "FFVars_Com (Cmt act P) = fvars act \<union> (FFVars P - bvars act)"
+lemma FFVars_comP_Cmt: "FFVars_comP (Cmt act P) = fvars act \<union> (FFVars P - bvars act)"
   by (cases act) auto
 
 lemma empty_bvars_vars_fvars: "bvars act = {} \<Longrightarrow> vars act = fvars act"
@@ -77,14 +77,14 @@ proof-
     using finite_Tsupp by blast
   then obtain x where "x \<notin> set xs \<union> Tsupp x1 x2"
     by (meson ex_new_if_finite finite_iff_le_card_var
-        infinite_iff_natLeq_ordLeq var_Proc_pre_class.large)
+        infinite_iff_natLeq_ordLeq var_procP_pre_class.large)
   thus ?thesis by auto
 qed
 
 lemma Bout_inject: "(Bout x y t = Bout x' y' t') \<longleftrightarrow>
   x = x' \<and>
   (\<exists>f. bij f \<and> |supp (f::var \<Rightarrow> var)| <o |UNIV::var set|
-  \<and> id_on (FFVars_Proc t - {y}) f \<and> f y = y' \<and> rrename_Proc f t = t')"
+  \<and> id_on (FFVars_procP t - {y}) f \<and> f y = y' \<and> rrename_procP f t = t')"
   by (auto 0 4 simp: id_on_def intro!: exI[of _ "id(y:=y', y':=y)"] rrename_cong)
 declare Bout_inj[simp del]
 
@@ -107,7 +107,7 @@ lemma bvars_rrename_bound_action[simp]: "bvars (rrename_bound_action f \<alpha>)
 lemma Cmt_rrename_bound_action: "bij (f :: var \<Rightarrow> var) \<Longrightarrow> |supp f| <o |UNIV :: var set| \<Longrightarrow> id_on (FFVars P - bvars \<alpha>) f \<Longrightarrow>
   Cmt \<alpha> P = Cmt (rrename_bound_action f \<alpha>) (rrename f P)"
   by (cases \<alpha>)
-    (force simp: Bout_inject id_on_def intro!: exI[of _ f] Proc.rrename_cong_ids[symmetric] rrename_cong)+
+    (force simp: Bout_inject id_on_def intro!: exI[of _ f] procP.rrename_cong_ids[symmetric] rrename_cong)+
 
 lemma Cmt_rrename_bound_action_Par: "bij (f :: var \<Rightarrow> var) \<Longrightarrow> |supp f| <o |UNIV :: var set| \<Longrightarrow> id_on (FFVars P \<union> FFVars Q - bvars \<alpha>) f \<Longrightarrow>
   Cmt \<alpha> (P \<parallel> Q) = Cmt (rrename_bound_action f \<alpha>) (rrename f P \<parallel> rrename f Q)"
