thys/Pi_Calculus/Pi_cong.thy
@@ -6,7 +6,7 @@ abbreviation Tsupp :: "proc \<Rightarrow> proc \<Rightarrow> var set" where
   "Tsupp e1 e2 \<equiv> FFVars e1 \<union> FFVars e2"
 
 lemma fresh: "\<exists>xx. xx \<notin> Tsupp (t :: proc) t2"
-  by (metis (no_types, lifting) exists_var finite_iff_le_card_var Proc.Un_bound Proc.set_bd_UNIV)
+  by (metis (no_types, lifting) exists_var finite_iff_le_card_var procP.Un_bound procP.set_bd_UNIV)
 
 (* Structural congurence *)
 binder_inductive cong :: "proc \<Rightarrow> proc \<Rightarrow> bool" (infix "(\<equiv>\<^sub>\<pi>)" 40) where
@@ -21,7 +21,7 @@ binder_inductive cong :: "proc \<Rightarrow> proc \<Rightarrow> bool" (infix "(\
   subgoal for R B \<sigma> x1 x2
     apply simp
     by (elim disj_forward case_prodE)
-      (auto simp: isPerm_def Proc.rrename_comps
+      (auto simp: isPerm_def procP.rrename_comps
         | ((rule exI[of _ "\<sigma> _"] exI)+, (rule conjI)?, rule refl)
         | ((rule exI[of _ "\<sigma> _"])+; auto))+
   subgoal premises prems for R B x1 x2
@@ -40,7 +40,7 @@ thm cong.strong_induct
 thm cong.equiv
 
 lemma finite_Tsupp: "finite (Tsupp x1 x2)"
-  by (metis FFVars_Com_simps(5) finite_FFVars_Com finite_Un)
+  by (metis FFVars_comP_simps(5) finite_FFVars_comP finite_Un)
 
 lemma exists_fresh:
   "\<exists> z. z \<notin> set xs \<and> (z \<notin> Tsupp x1 x2)"
@@ -50,7 +50,7 @@ proof-
     using finite_Tsupp by blast
   then obtain x where "x \<notin> set xs \<union> Tsupp x1 x2"
     by (meson ex_new_if_finite finite_iff_le_card_var
-        infinite_iff_natLeq_ordLeq var_Proc_pre_class.large)
+        infinite_iff_natLeq_ordLeq var_procP_pre_class.large)
   thus ?thesis by auto
 qed
 
@@ -62,15 +62,15 @@ binder_inductive trans :: "proc \<Rightarrow> proc \<Rightarrow> bool" (infix "(
   subgoal for R B \<sigma> x1 x2
     apply simp
     apply (elim disj_forward exE)
-       apply  (auto simp: isPerm_def Proc.rrename_comps
+       apply  (auto simp: isPerm_def procP.rrename_comps
         | ((rule exI[of _ "\<sigma> _"] exI)+, (rule conjI)?, rule refl)
         | ((rule exI[of _ "\<sigma> _"])+; auto))+
-    by (metis cong.equiv bij_imp_inv' Proc.rrename_bijs Proc.rrename_inv_simps)
+    by (metis cong.equiv bij_imp_inv' procP.rrename_bijs procP.rrename_inv_simps)
   subgoal for R B x1 x2
     unfolding ex_push_inwards conj_disj_distribL ex_disj_distrib ex_simps(1,2)[symmetric]
       ex_comm[where P = P for P :: "_ set \<Rightarrow> _ \<Rightarrow> _"]
     apply (elim disj_forward exE; simp; clarsimp)
-      apply (auto simp only: fst_conv snd_conv Proc.set)
+      apply (auto simp only: fst_conv snd_conv procP.set)
     subgoal for x z P y Q
       apply (rule exE[OF exists_fresh[of "[x, y, z]" P Q]])
       subgoal for w
