thys/Untyped_Lambda_Calculus/LC_Beta.thy
@@ -7,7 +7,7 @@ begin
 abbreviation Tsupp where "Tsupp a b \<equiv> FFVars a \<union> FFVars b"
 lemma fresh: "\<exists>xx. xx \<notin> Tsupp (t1::lterm) t2"
   unfolding prod.collapse
-   by (metis (no_types, lifting) exists_var finite_iff_le_card_var Lterm.Un_bound Lterm.set_bd_UNIV)
+   by (metis (no_types, lifting) exists_var finite_iff_le_card_var ltermP.Un_bound ltermP.set_bd_UNIV)
 
 binder_inductive step :: "lterm \<Rightarrow> lterm \<Rightarrow> bool" where
   Beta: "step (Ap (Lm x e1) e2) (tvsubst (Vr(x:=e2)) e1)"
@@ -16,7 +16,7 @@ binder_inductive step :: "lterm \<Rightarrow> lterm \<Rightarrow> bool" where
 | Xi: "step e e' \<Longrightarrow> step (Lm x e) (Lm x e')"
   subgoal for \<sigma> R B t  \<comment> \<open>equivariance\<close>
     by (elim disj_forward case_prodE)
-      (auto simp: isPerm_def Lterm.rrename_comps rrename_tvsubst_comp
+      (auto simp: isPerm_def ltermP.rrename_comps rrename_tvsubst_comp
          | ((rule exI[of _ "\<sigma> _"] exI)+, (rule conjI)?, rule refl)
          | ((rule exI[of _ "\<sigma> _"])+; auto))+
   subgoal premises prems for R B x1 x2  \<comment> \<open>refreshability\<close>
